src/drf/PromiseFree.v
@@ -172,7 +172,7 @@ Qed.
 Lemma key_lemma
       cS1 cT1 cS2 cT2 tid
       (PI_CONSISTENT : pi_consistent (cS1, cT1))
-      (WF : pi_wf eq (cS1, cT1))
+      (WF : pi_wf loctmeq (cS1, cT1))
       (RACEFREE : pf_racefree cS1)
       (STEPS : rtc (pi_step_evt true tid) (cS1, cT1) (cS2, cT2))
       loc ts 
@@ -180,20 +180,31 @@ Lemma key_lemma
       (THREAD2 : IdentMap.find tid (Configuration.threads cT2) = Some (lst2, lc2))
       (PROMISE2 : Memory.get loc ts (Local.promises lc2) = Some (from2, msg2))
       cSTM3
-      (STEPS_LIFT : rtc (pi_step_lift_except loc ts tid) (cS2, cT2, cT2.(Configuration.memory)) cSTM3)
-      cM4 pre
-      (PI_STEPS : with_pre (small_step false tid) (conf_update_memory cSTM3.(fst).(snd) cSTM3.(snd)) pre cM4)
-      (PRCONSIS: promise_consistent_th tid cM4)
-      lst4 lc4
-      (THREAD4 : IdentMap.find tid (Configuration.threads cM4) = Some (lst4, lc4))
-      (TIMELT: Time.lt (lc4.(Local.commit).(Commit.cur).(Capability.rw) loc) ts)
-  : 
-  exists cS4 pre',
-  <<STEPS: with_pre (pi_step false tid) (cSTM3.(fst).(fst), conf_update_memory cSTM3.(fst).(snd) cSTM3.(snd)) pre' (cS4, cM4)>>
-  /\
-  <<EQPRE: pre = pi_pre_proj pre'>>.
+      (STEPS_LIFT : rtc (pi_step_lift_except loc ts tid) (cS2, cT2, cT2.(Configuration.memory)) cSTM3):
+  exists msgs,
+  <<EQMEM: mem_eqrel (Capability_lift_le loc ts msgs) cSTM3.(fst).(snd).(Configuration.memory) cSTM3.(snd)>> /\
+  <<IN: Memory.get loc ts cSTM3.(fst).(snd).(Configuration.memory) <> None>> /\
+  <<MAIN:
+      forall cM4 pre
+        (PI_STEPS : with_pre (small_step false tid) (conf_update_memory cSTM3.(fst).(snd) cSTM3.(snd)) pre cM4)
+        (PRCONSIS: promise_consistent_th tid cM4)
+        lst4 lc4
+        (THREAD4 : IdentMap.find tid (Configuration.threads cM4) = Some (lst4, lc4))
+        (TIMELT: Time.lt (lc4.(Local.commit).(Commit.cur).(Capability.rw) loc) ts),
+    <<NOMSG: match pre with 
+             | Some (_,pe) => 
+               match ThreadEvent.is_reading pe with
+               | Some (l, t, val, relr, ordr) => ~ List.In (l,t) msgs
+               | _ => True
+               end
+             | _ => True 
+             end>> /\
+    exists cS4 pre',
+    <<STEPS: with_pre (pi_step false tid) (cSTM3.(fst).(fst), conf_update_memory cSTM3.(fst).(snd) cSTM3.(snd)) pre' (cS4, cM4)>>
+    /\
+    <<EQPRE: pre = pi_pre_proj pre'>> >>.
 Proof.
-  assert (WF2: pi_wf eq (cS2,cT2)).
+  assert (WF2: pi_wf loctmeq (cS2,cT2)).
   { eapply rtc_pi_step_future; eauto.
     eapply rtc_implies, STEPS; eauto. }
   move WF2 after STEPS_LIFT.
@@ -202,10 +213,18 @@ Proof.
   apply Operators_Properties.clos_rt_rt1n_iff, 
         Operators_Properties.clos_rt_rtn1_iff in STEPS_LIFT.
   induction STEPS_LIFT.
-  { s. i. destruct cT2. unfold conf_update_memory in *. ss.
-    eapply with_pre_implies in PI_STEPS.
-    - exploit pi_consistent_rtc_small_step_pi; try eapply WF; eauto.
-    - i. inv STEP. eauto. }
+  { exists []. splits.
+    - s. split; ii; esplits; eauto.
+    - s. inv WF2. inv WFT. inv WF0.
+      destruct lst2. exploit THREADS; eauto.
+      intro X. inv X. apply PROMISES in PROMISE2. rewrite PROMISE2. done.
+    - s. i. split. 
+      { destruct pre; eauto. destruct p; eauto. destruct (ThreadEvent.is_reading t0); repeat destruct p; eauto. }
+      destruct cT2. unfold conf_update_memory in *. ss.
+      eapply with_pre_implies in PI_STEPS.
+      + exploit pi_consistent_rtc_small_step_pi; try eapply WF; eauto.
+      + i. inv STEP. eauto. 
+  }
 
   apply Operators_Properties.clos_rt_rtn1_iff, 
         Operators_Properties.clos_rt_rt1n_iff in STEPS_LIFT.
@@ -214,20 +233,24 @@ Proof.
   destruct z as [[cS4 cT4] M4].
   rename H into PSTEP. ss.
 
-  assert (WF3: pi_wf eq (cS3, cT3)).
+  assert (WF3: pi_wf loctmeq (cS3, cT3)).
   { eapply rtc_pi_step_future; eauto.
     eapply pi_steps_lift_except_pi_steps in STEPS_LIFT.
     eapply rtc_implies, STEPS_LIFT.
     i. inv PR. eauto. }
 
-  assert (WF4: pi_wf eq (cS4, cT4)).
-  { inv PSTEP. eapply pi_step_future; eauto. }
-  
+  assert (WF4: pi_wf loctmeq (cS4, cT4)).
+  { inv PSTEP. inv USTEP. eapply pi_step_future; eauto. }
+
+  des. inv PSTEP. rename USTEP into PSTEP.
+  exploit pi_step_lift_except_future; try apply PSTEP; eauto.
+  i; des. clear MEMFUT TIMELE.
+  esplits; eauto.
+
   s. i. assert (X := PSTEP). inv X. rename cM4 into cM4'.
 
   hexploit rtc_pi_step_lift_except_find; eauto. 
   s; intro THEQA; des.
-
 
   hexploit rtc_pi_step_lift_except_find.
   { econs 2; [|reflexivity]. eauto. }
@@ -235,7 +258,15 @@ Proof.
 
   rewrite <-THEQB0,<-THEQA0, THREAD2 in FIND. inv FIND.
 
-  cut ((exists cS3' cM3' lst3' com3' com4' prm3',
+  cut((match pre with
+       | Some (_, pe) =>
+         match ThreadEvent.is_reading pe with
+         | Some (l, t0, _, _, _) => ~ List.In (l, t0) (msg_add e msgs)
+         | None => True
+         end
+       | None => True
+       end) /\
+      (exists cS3' cM3' lst3' com3' com4' prm3',
        <<STEPS3: rtc (pi_step_evt false tid) (cS3, conf_update_memory cT3 M3) (cS3',cM3')>> /\
        <<MEMLE: mem_eqlerel_lift loc ts prm3' k e cM3'.(Configuration.memory) cM4'.(Configuration.memory)>> /\
        <<SCLE: TimeMap.le cM3'.(Configuration.sc) cM4'.(Configuration.sc)>> /\
@@ -245,12 +276,13 @@ Proof.
        (exists cS4' pre',
        <<STEPS4: with_pre (pi_step false tid) (cS4, conf_update_memory cT4 M4) pre' (cS4',cM4')>>/\
        <<EQPRE: pre = pi_pre_proj pre'>>)).
-  { i; des. exists cS4'; esplits; eauto. }
+  { i; des. eauto. }
 
   move cM4' at bottom. move lst4 at bottom. move lc4 at bottom. move TIMELT at bottom.
   revert_until PI_STEPS.
   induction PI_STEPS; i.
-  { destruct lc4 as [com4 prm4]. subst. ss.
+  { split; eauto. 
+    destruct lc4 as [com4 prm4]. subst. ss.
     esplits.
     { eauto. }
     { econs; eauto.
@@ -272,12 +304,16 @@ Proof.
   assert (STEP2 := PSTEP0). inv PSTEP0. ss.
   rewrite IdentMap.gss in THREAD4. depdes THREAD4.
 
-  assert (WF3':= rtc_pi_step_lift_except_wf WF2 STEPS_LIFT). ss.
+  assert (MGET: Memory.get loc ts (Configuration.memory cT2) <> None).
+  { inv WF2. inv WFT. inv WF0. destruct lst.
+    hexploit THREADS; eauto.
+    intro X. inv X. apply PROMISES in PROMISE2. rewrite PROMISE2. done. }
 
-  hexploit rtc_pi_step_lift_except_wf; swap 1 2.
-  { etrans; [eauto|]. econs 2; [|reflexivity]. eauto. }
-  { eauto. }
-  s. intro WF4'.
+  exploit conf_update_memory_wf; try apply EQMEM; eauto.
+  intro WF3'.
+
+  exploit conf_update_memory_wf; try apply EQMEM0; eauto.
+  intro WF4'.
 
   hexploit rtc_small_step_future; swap 1 2.
   { eapply rtc_implies, with_pre_rtc_step_union, PI_STEPS. eauto. }
@@ -293,27 +329,24 @@ Proof.
   i; des. subst. clear IHPI_STEPS.
   rewrite THS4 in TID0. depdes TID0.
 
-  exploit rtc_pi_step_future; swap 1 2.
+  exploit rtc_pi_step_future; swap 1 3; swap 2 3.
   { eapply rtc_implies, STEPS3. eauto. }
+  { eauto. }
   { eauto. }
   intros [SEMI_WF3 _]. des.
 
-  exploit rtc_pi_step_future; swap 1 2.
+  exploit rtc_pi_step_future; swap 1 3; swap 2 3.
   { eapply rtc_implies, with_pre_rtc_step_union, STEPS4. eauto. }
+  { eauto. }
   { eauto. }
   intros [SEMI_WF4 _]. des.
 
-  exploit (@lift_step _ (Thread.mk _ st1 (Local.mk com3' prm3') cM3'.(Configuration.sc) cM3'.(Configuration.memory))); [apply STEP|..]; eauto.
-  { admit. (* Local.wf *) }
-  { admit. (* Local.wf *) }
-  { admit. (* sc is closed w.r.t. mem *) }
-  { admit. (* sc is closed w.r.t. mem *) }
-  { admit. (* mem is closed *) }
-  { admit. (* mem is closed *) }
-  i; des.
-
-  (* Read the message "e" *)
-  { destruct (Loc.eq_dec loc loc0) eqn: NEQ.
+  assert(IMP: forall loc0 ts0 from valr valw relr relw ordr ordw
+                (EVTR : ThreadEvent.is_reading e0 = Some (loc0, ts0, valr, relr, ordr))
+                (EVTW : ThreadEvent.is_writing e = Some (loc0, from, ts0, valw, relw, ordw)),
+              False).
+  { (* Read the message "e" *)
+    i. destruct (Loc.eq_dec loc loc0) eqn: NEQ.
     { exfalso. subst. inv PI_STEP.
       destruct lst.
       eapply NOWR; eauto.
@@ -361,8 +394,8 @@ Proof.
         + eauto.
       - eauto.
     }
+    i; des. 
 
-    i; des. exfalso.
     inv MEMLE. r in MEMWR. rewrite EVTW in MEMWR. des. rewrite NEQ in PMREL.
     inv STEP; inv STEP0; inv EVTR.
     - move TIMELT at bottom. move LOCAL at bottom. move PMREL at bottom. move ORDR at bottom.
@@ -370,6 +403,17 @@ Proof.
     - move TIMELT at bottom. move LOCAL1 at bottom. move LOCAL2 at bottom. move PMREL at bottom. move ORDR at bottom.
       admit. (* jeeoon easy; PMREL, TIMELT, LOCAL1, LOCAL2, ORDR *)
   }
+
+  exploit (@lift_step _ (Thread.mk _ st1 (Local.mk com3' prm3') cM3'.(Configuration.sc) cM3'.(Configuration.memory))); [apply STEP|..]; eauto.
+  { inv SEMI_WF3. inv WFT. inv WF0. s. eapply THREADS. eauto. }
+  { inv SEMI_WF4. inv WFT. inv WF0. s. eapply THREADS. eauto. }
+  { s. inv SEMI_WF3. inv WFT. eauto. }
+  { s. inv SEMI_WF4. inv WFT. eauto. }
+  { s. inv SEMI_WF3. inv WFT. eauto. }
+  { s. inv SEMI_WF4. inv WFT. eauto. }
+  i; des.
+
+  { exfalso. eauto. }
 
   (* Simulation exists *)  
   assert (NOPRMEVT: ThreadEvent_is_promising eS = None).
@@ -381,7 +425,7 @@ Proof.
   intros STEPS3'.
   eapply rtc_step_union_with_pre in STEPS3'. des.
 
-  exploit (@IHSTEPS_LIFT (Configuration.mk (IdentMap.add tid (existT _ _ st2, lcx) cM3'.(Configuration.threads)) scx mx)); s; swap 1 3; swap 2 3.
+  exploit (@MAIN (Configuration.mk (IdentMap.add tid (existT _ _ st2, lcx) cM3'.(Configuration.threads)) scx mx)); s; swap 1 3; swap 2 3.
   { rewrite IdentMap.gss. eauto. }
   { eapply with_pre_trans.
     - apply STEPS3'.
@@ -403,6 +447,20 @@ Proof.
   destruct lcx as [comx prmx].
   destruct lc4 as [com4 prm4].
   ss. subst.
+
+  apply strengthen.
+  split. 
+  { destruct (ThreadEvent.is_reading e0) as [[[[[]]]]|] eqn: EVTR; eauto.
+    unfold msg_add.
+    assert (NIN: ~ List.In (t,t0) msgs).
+    { destruct eS; inv EVT; inv EVTR; eauto. }
+
+    destruct (ThreadEvent.is_writing e) as [[[[[[]]]]]|] eqn: EVTW; eauto.
+    apply List.not_in_cons; split; eauto.
+    intro X; inv X. eauto.
+  }
+
+  intro NOTIN.
   split.
   { esplits; [by eapply with_pre_rtc_step_union, STEPS0|..]; eauto.
     { s. rewrite IdentMap.gss. eauto. }
@@ -444,15 +502,19 @@ Proof.
         eapply Local.step_read; cycle 1; eauto.
         
         inv STEPS0.
-        hexploit rtc_pi_step_future; swap 1 2.
+        hexploit rtc_pi_step_future; swap 1 3; swap 2 3.
         { eapply rtc_implies, with_pre_rtc_step_union, PSTEPS. eauto. }
-        { eapply rtc_pi_step_lift_except_wf with (cSTM2:=(_,_,_)); [by apply WF2|]. eauto. }
+        { eauto. }
+        { eauto. }
         s; intros [PIWF0 _]. inv PIWF0.
 
         ss. des. subst. inv EVT. inv PSTEP0. inv STEPS0. inv STEP; inv STEP1. inv LOCAL0. ss.
         exploit LR0; eauto. i; des.
 
-        eapply RL; eauto.
+        hexploit RL; [by eauto|..]; cycle 1.
+        { i. des. rdes CMP0; subst; eauto.
+          exfalso. apply NOTIN; eauto. }
+
         intros tid1 PRM4. apply (NOT tid1).
         destruct (Ident.eq_dec tid1 tid) eqn: TEQ.
         { subst. inv PRM4. rewrite THS4 in TID1. inv TID1.
@@ -478,8 +540,8 @@ Proof.
   }
 
   (* Write step *)
-  { hexploit local_simul_write; try apply LOCAL.
-    { inv SEMI_WF4. ii. apply LR in IN. des. esplits; eauto. }
+  { hexploit (@local_simul_write (Capability_lift_le loc ts (msg_add e msgs))); try apply LOCAL.
+    { inv SEMI_WF4. ii. apply LR in IN1. des. esplits; eauto. }
     { admit. (* memory & promises are disjoint *) }
     intro WRITE4. des.
 
@@ -512,8 +574,8 @@ Proof.
   (* Update step *)
   { assert (X:= LOCAL1). inv X. ss.
 
-    hexploit local_simul_write; try apply LOCAL2. 
-    { inv SEMI_WF4. ii. apply LR in IN. des. esplits; eauto. }
+    hexploit (@local_simul_write (Capability_lift_le loc ts (msg_add e msgs))); try apply LOCAL2. 
+    { inv SEMI_WF4. ii. apply LR in IN1. des. esplits; eauto. }
     { admit. (* memory & promises are disjoint *) }
     intro WRITE4. des.
     
@@ -532,15 +594,19 @@ Proof.
           eapply Local.step_read; cycle 1; eauto.
           
           inv STEPS0.
-          hexploit rtc_pi_step_future; swap 1 2.
+          hexploit rtc_pi_step_future; swap 1 3; swap 2 3.
           { eapply rtc_implies, with_pre_rtc_step_union, PSTEPS. eauto. }
-          { eapply rtc_pi_step_lift_except_wf with (cSTM2:=(_,_,_)); [by apply WF2|]. eauto. }
+          { eauto. }
+          { eauto. }
           s; intros [PIWF0 _]. inv PIWF0.
 
           ss. des. subst. inv EVT. inv PSTEP0. inv STEPS0. inv STEP; inv STEP1. inv LOCAL0. ss.
           exploit LR0; eauto. i; des.
 
-          eapply RL; eauto.
+          hexploit RL; [by eauto|..]; cycle 1.
+          { i. des. rdes CMP0; subst; eauto.
+            exfalso. apply NOTIN; eauto. }
+
           intros tid1 PRM4. apply (NOT tid1).
           destruct (Ident.eq_dec tid1 tid) eqn: TEQ.
           { subst. inv PRM4. rewrite THS4 in TID1. inv TID1.
@@ -612,14 +678,14 @@ Proof.
     }
     eauto.
   }
-Admitted. (* jeehoo: very easy *)
+Admitted. (* jeehoon: very easy *)
 
 Theorem pi_consistent_pi_step_pi_consistent
       cST1 cST2 tid
       (PI_CONSISTENT: pi_consistent cST1)
       (CONSISTENT: Configuration.consistent cST1.(snd))
       (PI_RACEFREE: pf_racefree cST1.(fst))
-      (WF: pi_wf cST1)
+      (WF: pi_wf loctmeq cST1)
       (STEP: rtc (pi_step_evt true tid) cST1 cST2)
       (CONSISTENT2: Configuration.consistent cST2.(snd)):
   pi_consistent cST2.
@@ -652,6 +718,7 @@ Proof.
   rename M2 into M3. ss.
 
   exploit rtc_pi_step_future; [eauto|..].
+  { reflexivity. }
   { eapply rtc_implies, STEP. i. inv PR. eauto. }
   i; des. ss. clear FUTURES FUTURET.
 
@@ -664,12 +731,14 @@ Proof.
   }
   destruct p as [[lang2 st2] lc2].
 
-  exploit pi_step_lift_except_future; eauto.
-  i. des. ss.
-
   exploit rtc_pi_step_lift_except_find; eauto.
   s; intro EQ; des. clear EQ.
   assert (X:= EQ0); rewrite THREAD, TH in X. depdes X.
+
+  exploit rtc_pi_step_lift_except_future; eauto.
+  { inv WF2. inv WFT. inv WF0. edestruct THREADS; eauto.
+    apply PROMISES in PROMISE. rewrite PROMISE. done. }
+  i. des. ss. rename WF0 into WF3.
 
   rewrite EQ0 in TH.
   exploit consistent_can_fulfill_promises_future; eauto.
@@ -680,12 +749,8 @@ Proof.
   exploit FULFILL; eauto.
   i; des. inv FULFILL1. clear FULFILL.
 
-  eapply rtc_step_union_with_pre in STEPS0. des.
-
-  assert (WF3:= rtc_pi_step_lift_except_wf WF2 STEPS_LIFT). ss.
-
   hexploit rtc_small_step_future; swap 1 2.
-  { eapply rtc_implies, with_pre_rtc_step_union, STEPS0. eauto. }
+  { eapply rtc_implies, STEPS0. eauto. }
   { inv WF3. eauto. }
   intros [WF4 _].
 
@@ -701,11 +766,18 @@ Proof.
 
   rewrite <-EQ0 in TH.
   exploit key_lemma; eauto.
+  s; i; des.
+  
+  exploit rtc_step_union_with_pre; [by apply STEPS0|].
+  intro STEPS'. des.
+
+  exploit (MAIN c0); eauto.
   { apply can_fulfill_promises_promise_consistent in FULFILL2; eauto.
     eapply promise_consistent_th_rtc_small_step, FULFILL2; eauto.
     etrans; [|apply STEPS1]. 
-    econs 2; [|reflexivity]. eauto. }
-  { eauto using small_step_write_lt. }
+    econs 2; [|reflexivity]; eauto.
+  }
+  { eapply small_step_write_lt; eauto. }
   s; i; des.
   
   exploit small_step_to_program_step_writing; eauto.
@@ -714,16 +786,13 @@ Proof.
   apply with_pre_rtc_step_union in STEPS2.
   exists cS4; esplits; eauto using (pi_steps_small_steps_fst false STEPS2).
 
-  hexploit rtc_pi_step_lift_except_wf; eauto.
-  s. intro WF3'.
-  
-  hexploit rtc_pi_step_future; [eauto|..]. 
+  exploit rtc_pi_step_future; [apply WF3|..].
+  { reflexivity. }
   { eapply rtc_implies, STEPS2. eauto. }
-  s. intros [WF4' _].
-  
-  inv WF4'. inv EVENT0.
+  i; des.
+
+  inv WF0. inv EVENT0.
   econs; eauto.
   by rewrite THS; setoid_rewrite IdentMap.Properties.F.map_o; rewrite TH0.
-Grab Existential Variables. eauto. eauto. eauto.
 Qed.
 
